feat: basic nunchaku reduction

Nunchaku/Util/NunchakuBuilder.lean
@@ -6,4 +6,20 @@ This module contains utility functions for building Nunchaku syntax and problems
 
 namespace Nunchaku
 
+def NunType.ofList (types : List NunType) (h : types ≠ []) : NunType :=
+  let revTypes := types.reverse
+  let output := revTypes.head (by simp [h, revTypes])
+  let remainder := revTypes.tail
+  remainder.foldl (init := output) (fun acc typ => .arrow typ acc)
+
+def NunTerm.not (arg : NunTerm) : NunTerm := .app (.builtin .not) arg
+def NunTerm.and (lhs rhs : NunTerm) : NunTerm := .app (.app (.builtin .and) lhs) rhs
+def NunTerm.or (lhs rhs : NunTerm) : NunTerm := .app (.app (.builtin .or) lhs) rhs
+def NunTerm.eq (lhs rhs : NunTerm) : NunTerm := .app (.app (.builtin .eq) lhs) rhs
+def NunTerm.neq (lhs rhs : NunTerm) : NunTerm := .app (.app (.builtin .neq) lhs) rhs
+def NunTerm.equiv (lhs rhs : NunTerm) : NunTerm := .app (.app (.builtin .equiv) lhs) rhs
+def NunTerm.imply (lhs rhs : NunTerm) : NunTerm := .app (.app (.builtin .imply) lhs) rhs
+def NunTerm.ite (discr lhs rhs : NunTerm) : NunTerm :=
+  .app (.app (.app (.builtin .ite) discr) lhs) rhs
+
 end Nunchaku
