Nunchaku/Transformation/Falsify.lean
@@ -1,0 +1,27 @@
+import Nunchaku.Util.Pipeline
+import Nunchaku.Util.Model
+
+/-!
+This module contains the transformation for negating the goal should that be necessary.
+-/
+
+namespace Nunchaku
+namespace Transformation
+namespace Falsify
+
+def transformation : Transformation Lean.MVarId Lean.MVarId LeanResult LeanResult where
+  st := Unit
+  inner := {
+    name := "Falsify"
+    encode g := g.withContext do
+      if (← read).falsify then
+        let g ← Lean.Meta.mkFreshExprMVar (Lean.mkNot (← g.getType))
+        return (g.mvarId!, ())
+      else
+        return (g, ())
+    decode _ res := return res
+  }
+
+end Falsify
+end Transformation
+end Nunchaku
