Nunchaku/Transformation/Output.lean
@@ -1,22 +1,380 @@
 import Nunchaku.Util.Pipeline
 import Nunchaku.Util.NunchakuSyntax
+import Nunchaku.Util.NunchakuBuilder
+import Nunchaku.Util.NunchakuPrinter
 import Nunchaku.Util.Model
+
+/-!
+This module contains the transformation for turning a monomorphized and dependently typed eliminated
+fragment of Lean into Nunchaku logic.
+-/
 
 namespace Nunchaku
 namespace Transformation
 namespace Output
 
+open Lean
+
+private inductive LeanIdentifier where
+  | goal
+  | assumption (fvar : FVarId)
+  | const (name : Name)
+  deriving BEq, Hashable, Repr, Inhabited
+
+private structure OutputContext where
+  /--
+  Identifies which part of the Lean context we are currently in to track dependencies
+  -/
+  currentIdent : LeanIdentifier
+  /--
+  The goal that we are serializing.
+  -/
+  goal : MVarId
+
+private structure OutputState where
+  /--
+  If `id2 ∈ dependencies[id1]` then the commands of `id2` need to come before the ones of `id1`
+  in the final Nunchaku problem.
+  -/
+  dependencies : Std.HashMap LeanIdentifier (List LeanIdentifier) := {}
+  /--
+  Worklist of remaining identifiers that need to be converted to Nunchaku commands.
+  -/
+  worklist : List LeanIdentifier
+  /--
+  Map from identifiers to Nunchaku commands that mirror their effect on the Nunchaku side.
+  -/
+  commands : Std.HashMap LeanIdentifier (List NunCommand) := {}
+  /--
+  Set of already visited identifiers in the fixpoint loop.
+  -/
+  visited : Std.HashSet LeanIdentifier := {}
+  /--
+  Counter used for fresh nunchaku variable identifiers.
+  -/
+  idCounter : Nat := 0
+
+
+private abbrev OutputM := ReaderT OutputContext <| StateRefT OutputState TransforM
+
+private def withCurrentIdent (id : LeanIdentifier) (x : OutputM α) : OutputM α :=
+  withReader (fun ctx => { ctx with currentIdent := id }) do
+    x
+
+private def getCurrentIdent : OutputM LeanIdentifier := return (← read).currentIdent
+
+private def isVisited (id : LeanIdentifier) : OutputM Bool := return (← get).visited.contains id
+private def markVisited (id : LeanIdentifier) : OutputM Unit :=
+  modify fun s => { s with
+    visited := s.visited.insert id,
+    dependencies := s.dependencies.alter id (some <| Option.getD · []),
+    commands := s.commands.alter id (some <| Option.getD · []),
+  }
+
+private def addCommand (cmd : NunCommand) : OutputM Unit := do
+  let id ← getCurrentIdent
+  let alter
+    | none => some [cmd]
+    | some cmds => some (cmd :: cmds)
+  modify fun s => { s with commands := s.commands.alter id alter }
+
+private def addCommands (cmds : List NunCommand) : OutputM Unit := do
+  let id ← getCurrentIdent
+  let alter
+    | none => some cmds
+    | some curr => some (cmds ++ curr)
+  modify fun s => { s with commands := s.commands.alter id alter }
+
+def addDepTo (ident : LeanIdentifier) : OutputM Unit := do
+  let currId ← getCurrentIdent
+  if currId == ident then
+    return
+  let alter
+    | none => some [ident]
+    | some curr => some (ident :: curr)
+  modify fun s => { s with dependencies := s.dependencies.alter currId alter }
+  if !(← get).visited.contains ident then
+    modify fun s => { s with worklist := ident :: s.worklist }
+
+def freshNunId : OutputM Nat := do
+  modifyGet fun s => (s.idCounter, { s with idCounter := s.idCounter + 1})
+
+private partial def OutputM.run (idents : List LeanIdentifier) (goal : MVarId) (handle : OutputM Unit) :
+    TransforM OutputState := do
+  let (_, st) ← StateRefT'.run (ReaderT.run go { currentIdent := .goal, goal }) { worklist := idents }
+  return st
+where
+  go : OutputM Unit := do
+    if let ident :: worklist := (← get).worklist then
+      modify fun s => { s with worklist }
+      if !(← isVisited ident) then
+        withCurrentIdent ident do
+          handle
+        markVisited ident
+      go
+    else
+      return ()
+
+private def mangleName (name : Lean.Name) : String :=
+  let comps := name.components.map (fun c => c.toString.replace "p" "pp")
+  String.intercalate "p" comps
+
+private def mangleAssumptionName (fvarId : FVarId) : MetaM String := do
+  return mangleName (← fvarId.getUserName)
+
+private partial def encodeType (expr : Lean.Expr) : OutputM NunType := do
+  let expr := (← instantiateMVars expr).consumeMData
+  go expr
+where
+  go (expr : Lean.Expr) : OutputM NunType := do
+    Meta.forallTelescope expr fun args output => do
+      let argsTypes ← args.mapM (Meta.inferType ·)
+      if argsTypes.any (fun t => t.hasAnyFVar (fun fvar => args.contains (.fvar fvar))) then
+        throwError m!"Cannot encode dependent type {expr}"
+      let encodeHeadType type := do
+        match type.consumeMData with
+        | .sort 0 => return .prop
+        | .sort (.succ _) => return .type
+        | .const name _ =>
+          addDepTo (.const name)
+          return .const (mangleName name)
+        | .fvar id =>
+          addDepTo (.assumption id)
+          return .const (← mangleAssumptionName id)
+        | .forallE .. => go type
+        | _ => throwError m!"Don't know how to encode {type} as output type"
+      let encodedArgsTypes ← argsTypes.mapM encodeHeadType
+      let encodeOutType type := do
+        match type.consumeMData with
+        | .sort 0 => return .prop
+        | .sort (.succ _) => return .type
+        | .const name _ =>
+          addDepTo (.const name)
+          return .const (mangleName name)
+        | .fvar id =>
+          addDepTo (.assumption id)
+          return .const (← mangleAssumptionName id)
+        | _ => throwError m!"Don't know how to encode {type} as output type"
+      let encodedOutType ← encodeOutType output
+      return .ofList (encodedArgsTypes.toList ++ [encodedOutType]) (by simp)
+
+private partial def encodeTerm (expr : Lean.Expr) : OutputM NunTerm := do
+  let expr ← instantiateMVars expr
+  go expr {}
+where
+  go (expr : Lean.Expr) (locals : FVarIdMap Nat) : OutputM NunTerm := do
+    match expr with
+    | .fvar fvarId =>
+      if let some nunId := locals.get? fvarId then
+        return .var nunId
+      else
+        addDepTo (.assumption fvarId)
+        return .const (← mangleAssumptionName fvarId)
+    | .const ``True [] => return .builtin .true
+    | .const ``False [] => return .builtin .false
+    | .const name _ =>
+      addDepTo (.const name)
+      return .const (mangleName name)
+    | .app fn arg =>
+      match_expr expr with
+      | Not p => return .not (← go p locals)
+      -- TODO Asserting
+      | And lhs rhs => return .and (← go lhs locals) (← go rhs locals)
+      | Or lhs rhs => return .or (← go lhs locals) (← go rhs locals)
+      | Eq _ lhs rhs => return .eq (← go lhs locals) (← go rhs locals)
+      | Ne _ lhs rhs => return .neq (← go lhs locals) (← go rhs locals)
+      | Iff lhs rhs => return .equiv (← go lhs locals) (← go rhs locals)
+      | ite _ discr _ lhs rhs =>
+        return .ite (← go discr locals) (← go lhs locals) (← go rhs locals)
+      | Exists ty prop =>
+        let encodedType ← encodeType ty
+        let argId ← freshNunId
+        if prop.isLambda then
+          Meta.lambdaBoundedTelescope prop 1 fun arg body => do
+            let arg := arg[0]!
+            let argType ← Meta.inferType arg
+            if argType.hasAnyFVar (fun fvar => locals.contains fvar) then
+              throwError m!"Can't encode dependent exists {expr}"
+            let locals := locals.insert arg.fvarId! argId
+            let encodedBody ← go body locals
+            return .exists argId encodedType encodedBody
+        else
+          -- TODO
+          throwError m!"Missing support for lambda free exists {expr}"
+      | _ => return .app (← go fn locals) (← go arg locals)
+    -- TODO: We can probably make these full telescopes
+    | .lam .. =>
+      Meta.lambdaBoundedTelescope expr 1 fun arg body => do
+        let arg := arg[0]!
+        let argType ← Meta.inferType arg
+        if argType.hasAnyFVar (fun fvar => locals.contains fvar) then
+          throwError m!"Can't encode dependent lambda {expr}"
+        let argId ← freshNunId
+        let locals := locals.insert arg.fvarId! argId
+        let encodedType ← encodeType argType
+        let encodedBody ← go body locals
+        return .lam argId encodedType encodedBody
+    | .forallE _ _ body _ =>
+      if (← Meta.inferType expr) != .sort 0 then
+        throwError m!"Can't encode forall in non Prop term {expr}"
+
+      -- If it doesn't it must be an implication
+      let properForall := body.hasLooseBVars
+      Meta.forallBoundedTelescope expr (some 1) fun arg body => do
+        let arg := arg[0]!
+        let argType ← Meta.inferType arg
+        if properForall then
+          if argType.hasAnyFVar (fun fvar => locals.contains fvar) then
+            throwError m!"Can't encode dependent forall {expr}"
+          let argId ← freshNunId
+          let locals := locals.insert arg.fvarId! argId
+          let encodedType ← encodeType argType
+          let encodedBody ← go body locals
+          return .forall argId encodedType encodedBody
+        else
+          let encodedLhs ← go argType locals
+          let encodedRhs ← go body locals
+          return .imply encodedLhs encodedRhs
+    | .letE .. =>
+      if !expr.letNondep! then
+        throwError m!"Can't encode dependent let {expr}"
+
+      Meta.letBoundedTelescope expr (some 1) fun arg body => do
+        let arg := arg[0]!
+        let argId ← freshNunId
+        let argFVar := arg.fvarId!
+        let locals := locals.insert argFVar argId
+        let encodedValue ← go ((← argFVar.getValue?).get!) locals
+        let encodedBody ← go body locals
+        return .let argId encodedValue encodedBody
+    | .mdata _ e => go e locals
+    -- TODO
+    | .proj .. => throwError "Missing support for projections"
+    | _ => throwError m!"Don't know how to encode term {expr}"
+
+private def encodeDataCtor (ctor : Name) : OutputM NunCtorSpec := do
+  let info ← getConstInfoCtor ctor
+  if info.numParams != 0 then
+    throwError "Inductive data type should be fully monomorphic at this point"
+  let args ← Meta.arrowDomainsN info.numFields info.type
+  let encodedArgs ← args.mapM encodeType
+  let mangled := mangleName ctor
+  return { name := mangled, arguments := encodedArgs.toList }
+
+private def LeanIdentifier.encode : OutputM Unit := do
+  match (← getCurrentIdent) with
+  | .goal =>
+    let statement ← (← read).goal.getType
+    trace[nunchaku.output] m!"Encoding the goal: {statement}"
+    let encoded ← encodeTerm statement
+    addCommand <| .goalDecl encoded
+  | .assumption fvar =>
+    trace[nunchaku.output] m!"Encoding fvar: {mkFVar fvar}"
+    let type ← fvar.getType
+    match ← Meta.inferType type with
+    | .sort 0 =>
+      -- `fvar` is a propositional assumption, we can interpret this as an axiom
+      let encoded ← encodeTerm type
+      addCommand <| .axiomDecl encoded
+    | .sort (.succ _) =>
+      -- `fvar` is some uninterpreted proper value, interpet it as such
+      let encoded ← encodeType type
+      let mangled := mangleName (← fvar.getUserName)
+      addCommand <| .valDecl mangled encoded
+    | ttype => throwError m!"Don't know how to handle {mkFVar fvar} : {type} : {ttype}"
+  | .const name =>
+    trace[nunchaku.output] m!"Encoding constant: {mkConst name}"
+    let constInfo ← getConstInfo name
+    match constInfo with
+    | .axiomInfo val =>
+      let encoded ← encodeTerm val.type
+      addCommand <| .axiomDecl encoded
+    | .defnInfo val =>
+      let eqns ← TransforM.getEquationsFor name
+      let encodedEqns ← eqns.mapM encodeTerm
+      let encodedType ← encodeType val.type
+      let mangled := mangleName name
+      addCommand <| .recDecl [{ name := mangled, type := encodedType, laws := encodedEqns }]
+    | .opaqueInfo val =>
+      let encodedType ← encodeType val.type
+      let mangled := mangleName name
+      addCommand <| .valDecl mangled encodedType
+    | .inductInfo val =>
+      match val.type with
+      | .sort (.succ _) =>
+        -- It's a regular inductive type
+        let mangled := mangleName name
+        let ctors ← val.ctors.mapM encodeDataCtor
+        addCommand <| .dataDecl [{ name := mangled, ctors }]
+      | _ =>
+        -- TODO: analyze if it is an inductive predicate (they can still have value args at this
+        -- point)
+        throwError s!"Don't know how to encode inductive {mkConst name}"
+    | .thmInfo val | .ctorInfo val | .recInfo val =>
+      trace[nunchaku.output] m!"Ignoring {val.name} as it should be irrelevant"
+      return ()
+    | .quotInfo _ => throwError "Cannot handle quotients"
+
+private structure TopoContext where
+  deps : Std.HashMap LeanIdentifier (List LeanIdentifier)
+  cmds : Std.HashMap LeanIdentifier (List NunCommand)
+
+private abbrev TopoM :=
+  ReaderT TopoContext <| StateT (Std.HashMap LeanIdentifier Bool) <| Except String
+
+private partial def OutputState.toProblem (state : OutputState) : Except String NunProblem :=
+  let deps := state.dependencies
+  let cmds := state.commands
+  let worklist := state.dependencies.keys
+  go worklist (Array.emptyWithCapacity cmds.size) |>.run { deps, cmds } |>.run' {}
+where
+  go (worklist : List LeanIdentifier) (acc : Array NunCommand) : TopoM NunProblem := do
+    match worklist with
+    | [] =>
+      let acc := acc ++ (← read).cmds[LeanIdentifier.goal]!
+      return { commands := acc.toList }
+    | elem :: worklist =>
+      let acc ← visit elem acc
+      go worklist acc
+
+  visit (elem : LeanIdentifier) (acc : Array NunCommand) : TopoM (Array NunCommand) := do
+    if elem == .goal then
+      return acc
+
+    if let some mark := (← get)[elem]? then
+      match mark with
+      | true => return acc
+      | false => throw "Graph has a cycle"
+
+    modify fun s => s.insert elem false
+
+    let mut acc := acc
+    for predecessor in (← read).deps[elem]! do
+      acc ← visit predecessor acc
+
+    modify fun s => s.insert elem true
+    return acc ++ (← read).cmds[elem]!
+
 def transformation : Transformation Lean.MVarId NunProblem NunResult LeanResult where
   st := Unit
   inner := {
     name := "Output"
-    encode g := return ({ commands := [] }, ())
+    encode g := g.withContext do
+      let mut idents := [.goal]
+      for decl in ← getLCtx do
+        if decl.isImplementationDetail then
+          continue
+        if decl.isLet then throwError "Let declarations not supported"
+        idents := .assumption decl.fvarId :: idents
+      let state ← OutputM.run idents g LeanIdentifier.encode
+      let problem ← IO.ofExcept state.toProblem
+      return (problem, ())
     decode _ res := do
       match res with
       | .unsat => return .unsat
       | .unknown => return .unknown
       -- TODO: proper model recovery
-      | .sat model => return .sat []
+      | .sat _ => return .sat []
   }
 
 
